cava/experiments/sv-experiments/indexing.cpp
@@ -1,0 +1,27 @@
+#include <stdlib.h>
+#include "Vindexing.h"
+#include "verilated.h"
+#include "verilated_vpi.h"
+#include "verilated_vcd_c.h"
+
+double main_time = 0;
+double sc_time_stamp() { return main_time; }
+
+int main(int argc, char **argv) {
+  Verilated::commandArgs(argc, argv);
+  Vindexing *top = new Vindexing;
+  VerilatedVcdC* vcd_trace = new VerilatedVcdC;
+  Verilated::traceEverOn(true);
+  top->trace(vcd_trace, 99);
+  top->eval(); vcd_trace->dump(main_time);
+  vcd_trace->open("nand2_tb.vcd");
+  for (unsigned int i = 0; i < 4; i++) {
+    top->clk = 0; main_time += 5;
+    top->eval(); vcd_trace->dump(main_time);
+    top->clk = 1;  main_time += 5;
+    top->eval(); vcd_trace->dump(main_time);
+  }
+  vcd_trace->close();
+  delete top;
+  exit(EXIT_SUCCESS);
+}
