cava/experiments/sv-experiments/indexing.sv
@@ -1,0 +1,91 @@
+// Copyright 2019 The Project Oak Authors
+//
+// Licensed under the Apache License, Version 2.0 (the "License");
+// you may not use this file except in compliance with the License.
+// You may obtain a copy of the License at
+//
+//     http://www.apache.org/licenses/LICENSE-2.0
+//
+// Unless required by applicable law or agreed to in writing, software
+// distributed under the License is distributed on an "AS IS" BASIS,
+// WITHOUT WARRANTIES OR CONDITIONS OF ANY KIND, either express or implied.
+// See the License for the specific language governing permissions and
+// limitations under the License.
+//
+
+module add4(
+  input logic[3:0] a,
+  input logic[3:0] b,
+  output logic[3:0] c
+);
+
+  assign c = a + b;
+
+endmodule
+
+module indexing(
+  input logic clk
+);
+
+  timeunit 1ns; timeprecision 1ns;
+
+  logic[7:0] wombat = 8'b10011100;
+  logic[2:0] iv = 3'd7;
+  logic bat1 = wombat[7];
+  logic bat2 = wombat[iv];
+  logic[2:0] sel = '{1'b1, 1'b1, 1'b1};
+  logic bat3 = wombat[sel];
+
+  logic[3:0] sum1;
+  logic[3:0] sum2;
+  logic[3:0] sum3;
+  logic[3:0] sum4;
+  logic[3:0] sum5;
+  logic[3:0] sums[2];
+
+  add4 av1 (.a(4'b0010), .b(4'b1100), .c(sum1));
+  add4 av2 (.a({1'b0, 1'b0, 1'b1, 1'b0}), .b(4'b1100), .c(sum2));
+
+  logic x[4] = '{1'b0, 1'b0, 1'b1, 1'b0};
+  logic y[4] = '{1'b1, 1'b0, 1'b0, 1'b0};
+
+  assign sum3 = {1'b0, 1'b0, 1'b1, 1'b0} + 'b1100;
+
+  assign sum4 = {1'b0, 1'b0, 1'b1, 1'b0} + 4'b1100;
+
+  assign sum5 = {x[0], x[1], x[2], x[3]} + 4'b1100;
+
+  logic[3:0] p = {1'b0, 1'b0, 1'b1, 1'b0};
+  logic[3:0] q = 4'b1100;
+
+  assign sums = '{p, q};
+
+  logic i1 = 1'b1;
+  logic i0 = 1'b0;
+  logic sel1 = 1'b1;
+  logic o;
+
+  logic[1:0] v0;
+  logic[0:0] v1;
+
+  assign o = v0[v1];
+  assign v1 = {sel1};
+  assign v0 = {i1,i0};
+
+
+  initial begin
+    $display("bat1 = %b", bat1);
+    $display("bat2 = %b", bat2);
+    $display("bat3 = %b", bat3);
+    $display("sum1 = %d", sum1);
+    $display("sum2 = %d", sum2);
+    $display("sum3 = %d", sum3);
+    $display("sum3 = %d", sum4);
+    $display("sum5 = %d", sum5);
+    $display("sums = %d %d", sums[0], sums[1]);
+    $display("v0 = %x", v0);
+    $display("v1 = %x", v1);
+    $display("o = %b", o);
+  end
+
+endmodule  
