cava/cava/Cava/Monad/CavaClass.v
@@ -14,13 +14,35 @@
 (* limitations under the License.                                           *)
 (****************************************************************************)
 
+From Coq Require Vector.
 Require Import ExtLib.Structures.Monads.
+
+From Cava Require Import Kind.
+
+Fixpoint denoteVecKind (bit: Type) (vec: Type -> nat -> Type) (k: Kind) : Type :=
+  match k with
+  | Bit => bit
+  | BitVec k2 s => vec (denoteVecKind bit vec k2) s
+  | _ => unit
+  end.
 
 (* The Cava class represents circuit graphs with Coq-level inputs and
    outputs, but does not represent the IO ports of circuits. This allows
    us to define both circuit netlist interpretations for the Cava class
    as well as behavioural interpretations for attributing semantics. *)
-Class Cava m bit `{Monad m} := {
+Class Cava m `{Monad m} bit (vec: Kind -> nat -> Type) := {
+  denoteKind: Kind -> Type;
+  denoteKindV: forall {k s}, denoteKind (BitVec k s) = vec k s;
+  vecBoolList: forall {s: nat}, Vector.t bit s -> vec Bit s;
+  vecList : forall {k: Kind} {s: nat}, Vector.t (denoteKind k) s ->
+            vec k s;
+  (* Convert a dynamic vector to a "static" list *)
+  vecToList: forall {k: Kind} {s: nat}, vec k s -> list (denoteKind k);
+  vecToVector: forall {k: Kind} {s: nat}, vec k s -> Vector.t (denoteKind k) s;
+  vecToVector1: forall {s: nat}, vec Bit s -> Vector.t bit s;
+  vecToVector2: forall {s: nat} (k2: Kind) (s2: nat), vec (BitVec k2 s2) s -> Vector.t (vec k2 s2) s;
+  defaultKind: forall {k: Kind}, @denoteKind k;
+  defaultBitVec : forall {sz}, vec Bit sz;          
   (* Constant values. *)
   zero : m bit; (* This component always returns the value 0. *)
   one : m bit; (* This component always returns the value 1. *)
@@ -47,9 +69,20 @@ Class Cava m bit `{Monad m} := {
          (bit * bit * bit * bit * bit * bit) -> m bit; (* 6-input LUT *)
   xorcy : bit * bit -> m bit; (* Xilinx fast-carry UNISIM with arguments O, CI, LI *)
   muxcy : bit -> bit -> bit -> m bit; (* Xilinx fast-carry UNISIM with arguments O, CI, DI, S *)
-  (* Synthesizable multiplexors *)
-  indexBitArray : list bit -> list bit -> m bit;
-  indexArray : list (list bit) -> list bit -> m (list bit);
+  (* Indexing is currently represented as a "circuit" but we may add features
+     to the SystemVerilog netlist generation back-end to allow these to me
+     functions rather than values in the monad type `m`.
+  *)
+  (* Dynamic indexing *)                                   
+  indexAt : forall {k: Kind} {sz isz: nat}, vec k sz -> vec Bit isz -> denoteKind k;
+  indexBitAt : forall {sz isz: nat}, vec Bit sz ->
+                                     vec Bit isz -> bit;
+  (* Static indexing *)
+  indexConst : forall {k: Kind} {sz: nat}, vec k sz -> nat -> denoteKind k;
+  indexBitConst : forall {sz: nat}, vec Bit sz -> nat -> bit;
+  slice : forall {k: Kind} {sz: nat} (startAt len: nat), vec k sz ->
+                 (startAt + len <= sz) -> vec k len;
   (* Synthesizable arithmetic operations. *)
-  unsignedAdd : list bit -> list bit -> m (list bit);
+  unsignedAdd : forall {a b : nat}, vec Bit a -> vec Bit b -> m (vec Bit (1 + max a b));
+  addNN : forall {a : nat}, vec Bit a -> vec Bit a -> m (vec Bit a);
 }.
