cava/cava/Cava/Monad/NetlistGeneration.v
@@ -15,64 +15,68 @@
 (****************************************************************************)
 
 From Coq Require Import Ascii String.
-From Coq Require Import Lists.List.
-Import ListNotations.
 Require Import ExtLib.Structures.Monads.
 Export MonadNotation.
 
+From Coq Require Import Vector.
 From Coq Require Import ZArith.
 
+From Coq Require Import Lists.List.
+Import ListNotations.
+
 Require Import Cava.Cava.
+Require Import Cava.VectorUtils.
 Require Import Cava.Monad.CavaClass.
 
+From Cava Require Import Kind.
 Require Import Cava.Signal.
 
 (******************************************************************************)
 (* Netlist implementations for the Cava class.                                *)
 (******************************************************************************)
 
-Definition invNet (i : Signal) : state CavaState Signal :=
+Definition invNet (i : Signal Bit) : state CavaState (Signal Bit) :=
   o <- newWire ;;
   addInstance (Not i o) ;;
   ret o.
 
-Definition andNet (i : Signal * Signal) : state CavaState Signal :=
+Definition andNet (i : Signal Bit * Signal Bit) : state CavaState (Signal Bit) :=
   let (i0, i1) := i in
   o <- newWire ;;
   addInstance (And i0 i1 o) ;;
   ret o.
 
-Definition nandNet (i : Signal * Signal) : state CavaState Signal :=
+Definition nandNet (i: Signal Bit * Signal Bit) : state CavaState (Signal Bit) :=
   let (i0, i1) := i in
   o <- newWire ;;
   addInstance (Nand i0 i1 o) ;;
   ret o.
 
-Definition orNet (i : Signal * Signal) : state CavaState Signal :=
+Definition orNet (i: Signal Bit * Signal Bit) : state CavaState (Signal Bit) :=
   let (i0, i1) := i in
   o <- newWire ;;
   addInstance (Or i0 i1 o) ;;
   ret o.
 
-Definition norNet (i : Signal * Signal) : state CavaState Signal :=
+Definition norNet (i: Signal Bit * Signal Bit) : state CavaState (Signal Bit) :=
   let (i0, i1) := i in
   o <- newWire ;;
   addInstance (Nor i0 i1 o) ;;
   ret o.
 
-Definition xorNet (i : Signal * Signal) : state CavaState Signal :=
+Definition xorNet (i: Signal Bit * Signal Bit) : state CavaState (Signal Bit) :=
   let (i0, i1) := i in
   o <- newWire ;;
   addInstance (Xor i0 i1 o) ;;
   ret o.
 
-Definition xnorNet (i : Signal * Signal) : state CavaState Signal :=
+Definition xnorNet (i: Signal Bit * Signal Bit) : state CavaState (Signal Bit) :=
   let (i0, i1) := i in
   o <- newWire ;;
   addInstance (Xnor i0 i1 o) ;;
   ret o.
 
-Definition bufNet (i : Signal) : state CavaState Signal :=
+Definition bufNet (i : Signal Bit) : state CavaState (Signal Bit) :=
   o <- newWire ;;
   addInstance (Buf i o) ;;
   ret o.
@@ -83,15 +87,15 @@ Definition bufNet (i : Signal) : state CavaState Signal :=
 
 Local Open Scope N_scope.
 
-Definition lut1Net (f : bool -> bool) (i : Signal) : state CavaState Signal :=
+Definition lut1Net (f : bool -> bool) (i : Signal Bit) : state CavaState (Signal Bit) :=
   let config := N.b2n (f false) + 2 * N.b2n (f true) in
   o <- newWire ;;
   addInstance (Component "LUT1" [("INIT", HexLiteral 2 config)]
                          [("O", o); ("I0", i)]) ;;
   ret o.
 
-Definition lut2Net (f : bool -> bool -> bool) (i : Signal * Signal) :
-           state CavaState Signal :=
+Definition lut2Net (f : bool -> bool -> bool) (i : Signal Bit * Signal Bit) :
+           state CavaState (Signal Bit) :=
   let config :=     N.b2n (f false false) +
                 2 * N.b2n (f true false) +
                 4 * N.b2n (f false true) + 
@@ -109,9 +113,9 @@ Definition f3List (f: bool -> bool -> bool -> bool) (l: list bool) : bool :=
   end.
 
 Definition lut3Net (f : bool -> bool -> bool -> bool)
-                   (i : Signal * Signal * Signal) : state CavaState Signal :=
+                   (i : Signal Bit * Signal Bit * Signal Bit) : state CavaState (Signal Bit) :=
   let powers := map (fun p => let bv := nat_to_list_bits_sized 3 (N.of_nat p) in
-                     2^(N.of_nat p) * N.b2n (f3List f bv)) (seq 0 8)  in
+                     2^(N.of_nat p) * N.b2n (f3List f bv)) (List.seq 0 8)  in
   let config := fold_left N.add powers 0 in
   let '(i0, i1, i2) := i in
   o <- newWire ;;
@@ -127,8 +131,8 @@ Definition f4List (f: bool -> bool -> bool -> bool -> bool) (l: list bool) :
   end.
 
 Definition lut4Net (f : bool -> bool -> bool -> bool -> bool)
-                   (i : Signal * Signal * Signal * Signal) :
-                  state CavaState Signal :=
+                   (i : Signal Bit * Signal Bit * Signal Bit * Signal Bit) :
+                  state CavaState (Signal Bit) :=
   let powers := map (fun p => let bv := nat_to_list_bits_sized 4 (N.of_nat p) in
                      2^(N.of_nat p) * N.b2n (f4List f bv)) (seq 0 16)  in
   let config := fold_left N.add powers 0 in
@@ -146,7 +150,7 @@ Definition f5List (f: bool -> bool -> bool -> bool -> bool -> bool)
   end.
 
 Definition lut5Net (f : bool -> bool -> bool -> bool -> bool -> bool)
-                  (i : Signal * Signal * Signal * Signal * Signal) : state CavaState Signal :=
+                  (i : Signal Bit * Signal Bit * Signal Bit * Signal Bit * Signal Bit) : state CavaState (Signal Bit) :=
   let powers := map (fun p => let bv := nat_to_list_bits_sized 5 (N.of_nat p) in
                      2^(N.of_nat p) * N.b2n (f5List f bv)) (seq 0 32)  in
   let config := fold_left N.add powers 0 in
@@ -164,7 +168,7 @@ Definition f6List (fn: bool -> bool -> bool -> bool -> bool -> bool -> bool)
   end.
 
 Definition lut6Net (f : bool -> bool -> bool -> bool -> bool -> bool -> bool)
-                  (i : Signal * Signal * Signal * Signal * Signal * Signal) : state CavaState Signal :=
+                  (i : Signal Bit * Signal Bit * Signal Bit * Signal Bit * Signal Bit * Signal Bit) : state CavaState (Signal Bit) :=
   let powers := map (fun p => let bv := nat_to_list_bits_sized 6 (N.of_nat p) in
                      2^(N.of_nat p) * N.b2n (f6List f bv)) (seq 0 64)  in
   let config := fold_left N.add powers 0 in
@@ -176,57 +180,78 @@ Definition lut6Net (f : bool -> bool -> bool -> bool -> bool -> bool -> bool)
 
 Local Close Scope N_scope.
 
-Definition xorcyNet (i : Signal * Signal) : state CavaState Signal :=
+Definition xorcyNet (i : Signal Bit * Signal Bit) : state CavaState (Signal Bit) :=
   let (ci, li) := i in
   o <- newWire ;;
   addInstance (Component "XORCY" [] [("O", o); ("CI", fst i); ("LI", snd i)]) ;;
   ret o.
 
-Definition muxcyNet (s ci di : Signal) : state CavaState Signal :=
+Definition muxcyNet (s ci di : Signal Bit) : state CavaState (Signal Bit) :=
   o <- newWire ;;
   addInstance ( Component "MUXCY" [] [("O", o); ("S", s); ("CI", ci); ("DI", di)]) ;;
   ret o.
 
-Definition indexBitArrayNet (i : list Signal) (sel : list Signal) :
-                            state CavaState Signal :=
-  o <- newWire ;;
-  addInstance (IndexBitArray i sel o) ;;
-  ret o.
-
-Definition indexArrayNet (i : list (list Signal)) (sel : list Signal) :
-                         state CavaState (list Signal) :=
-  let w := length (hd [] i) in (* The width of each bus *)
-  let m := length sel in       (* Number of bits to represent selector *)
-  let n := length i in         (* Number of values to select from *)
-  o <- newWires w ;;
-  addInstance (IndexArray i sel o) ;;
-  ret o.
-
-Definition unsignedAddNet (a : list Signal) (b : list Signal) :
-                          state CavaState (list Signal) :=
-  let sumSize := max (length a) (length b) + 1 in
-  sum <- newWires sumSize ;;
+Definition unsignedAddNet {m n : nat} 
+                          (a : Signal (BitVec Bit m)) (b : Signal (BitVec Bit n)) :
+                          state CavaState (Signal (BitVec Bit (1 + max m n))) :=
+  sum <- newVector Bit (1 + max m n) ;;
   addInstance (UnsignedAdd a b sum) ;;
   ret sum.
 
-Definition delayBitNet (i : Signal) : state CavaState Signal :=
+Definition addNNNet {m : nat} 
+                    (a : Signal (BitVec Bit m)) (b : Signal (BitVec Bit m)) :
+                    state CavaState (Signal (BitVec Bit m)) :=
+  sum <- newVector Bit m ;;
+  addInstance (UnsignedAdd a b sum) ;;
+  ret sum.
+
+Definition delayBitNet (i : Signal Bit) : state CavaState (Signal Bit) :=
   o <- newWire ;;
-  addSequentialInstance (DelayBit i o) ;;
+  addInstance (DelayBit i o) ;;
   ret o.
 
-Definition loopBitNet (A B : Type) (f : (A * Signal)%type -> state CavaState (B * Signal)%type) (a : A) : state CavaState B :=
+Definition loopBitNet (A B : Type) (f : (A * Signal Bit)%type -> state CavaState (B * Signal Bit)%type) (a : A) : state CavaState B :=
   o <- newWire ;;
   '(b, cOut) <- f (a, o) ;;
-  addInstance (AssignBit o cOut) ;;
+  assignSignal o cOut ;;
   ret b.
+
+Definition indexAtNet {k: Kind} {sz isz: nat}
+                      (v: Signal (BitVec k sz))
+                      (i: Signal (BitVec Bit isz)) :
+                      Signal k :=
+  IndexAt v i.                       
+
+Definition indexConstNet {k: Kind} {sz: nat}
+                         (v: Signal (BitVec k sz))
+                         (i: nat) :
+                         Signal k :=
+  IndexConst v i. 
+
+Definition sliceNet {k: Kind} {sz: nat}
+                    (startAt len: nat)
+                    (v: Signal (BitVec k sz)) :
+                    Signal (BitVec k len) :=
+  Slice startAt len v.                    
+
+Definition vecAsSignal (k: Kind) (s: nat) : Type := Signal (BitVec k s).
 
 (******************************************************************************)
 (* Instantiate the Cava class for CavaNet which describes circuits without    *)
 (* any top-level pins or other module-level data                              *)
 (******************************************************************************)
 
-Instance CavaNet : Cava (state CavaState) Signal :=
-  { zero := ret Gnd;
+Program Instance CavaNet : Cava (state CavaState) (Signal _) vecAsSignal :=
+  { denoteKind k := Signal k;
+    vecBoolList s l := VecLit l;
+    vecList k s l := VecLit l;
+    vecToList k s v := map (IndexConst v) (seq 0 s);
+    vecToVector k s v := Vector.map (IndexConst v) (vseq 0 s);
+    vecToVector1 s v := Vector.map (IndexConst v) (vseq 0 s);
+    vecToVector2 s k2 s2 v := Vector.map (IndexConst v) (vseq 0 s);
+    defaultKind := defaultKindSignal;
+    defaultBitVec sz := VecLit (Vector.const Gnd sz);
+    zero := ret Gnd;
     one := ret Vcc;
     delayBit := delayBitNet;
     loopBit a b := loopBitNet a b;
@@ -246,7 +271,12 @@ Instance CavaNet : Cava (state CavaState) Signal :=
     lut6 := lut6Net;
     xorcy := xorcyNet;
     muxcy := muxcyNet;
-    indexBitArray := indexBitArrayNet;
-    indexArray := indexArrayNet;
-    unsignedAdd := unsignedAddNet;
+    indexBitAt sz isz := @indexAtNet Bit sz isz;
+    indexAt k sz isz v sel := indexAtNet v sel;
+    indexConst k sz := indexConstNet;
+    indexBitConst sz := @indexConstNet Bit sz;
+    slice k sz start len v _ := @sliceNet k sz start len v;
+    unsignedAdd m n := @unsignedAddNet m n;
+    addNN m := @addNNNet m;
 }.
+
