cava/monad-examples/AdderTree.v
@@ -14,14 +14,15 @@
 (* limitations under the License.                                           *)
 (****************************************************************************)
 
-(* A codification of the Lava embedded DSL develope for Haskell into
-   Coq for the specification, implementaiton and formal verification of
-   circuits. Experimental work, very much in flux, as Satnam learns Coq!
-*)
-
+From Coq Require Import Program.Basics.
 From Coq Require Import Bool.Bool.
 From Coq Require Import Ascii String.
+From Coq Require Import NArith.
 Require Import Omega.
+
+From Coq Require Import Vector.
+From Coq Require Import Bool.Bvector.
+Import VectorNotations.
 
 From Coq Require Import Lists.List.
 Import ListNotations.
@@ -37,46 +38,64 @@ Require Import Cava.Monad.UnsignedAdders.
 (* by using the tree combinator.                                              *)
 (******************************************************************************)
 
-Definition adderTree {m bit} `{Cava m bit} := tree unsignedAdd.
+(* List based adder tree *)
+Definition adderTree {m bit vec} `{Cava m bit vec} {sz: nat}
+                     (n: nat) (v: vec (BitVec Bit sz) (2^(n+1))) :
+                      m (vec Bit sz) :=
+  let vv : Vector.t (vec Bit sz) (2^(n+1)) := vecToVector2 Bit sz v in                
+  tree addNN defaultBitVec n vv.
+
+(* Vector based adder tree which currently does not work *)
+Definition adderTreeV  {m bit vec} `{Cava m bit vec} {sz: nat}
+                       (n: nat) (v: vec (BitVec Bit sz) (2^(n+1))) :
+                       m (vec Bit sz) :=
+  let vv : Vector.t (vec Bit sz) (2^(n+1)) := vecToVector2 Bit sz v in                
+  treeV n addNN vv.
 
 (******************************************************************************)
 (* Some tests.                                                                *)
 (******************************************************************************)
 
-Definition v0 := nat_to_list_bits_sized 8  4.
-Definition v1 := nat_to_list_bits_sized 8 17.
-Definition v2 := nat_to_list_bits_sized 8  6.
-Definition v3 := nat_to_list_bits_sized 8  3.
+Definition v0 := N2Bv_sized 8  4.
+Definition v2 := N2Bv_sized 8  6.
+Definition v1 := N2Bv_sized 8 17.
+Definition v3 := N2Bv_sized 8  3.
 
 Local Open Scope N_scope.
 Local Open Scope string_scope.
 
 (* An adder tree with 2 inputs. *)
 
-Definition adderTree2 {m bit} `{Cava m bit} (v : list (list bit)) : m (list bit)
+Local Open Scope nat_scope.
+
+Definition adderTree2 {m bit vec} `{Cava m bit vec} {sz}
+                      (v : vec (BitVec Bit sz) 2) : m (vec Bit sz)
   := adderTree 0 v.
 
+Local Open Scope vector_scope.
+
 Definition v0_v1 := [v0; v1].
-Definition v0_plus_v1 : list bool := combinational (adderTree 0 v0_v1).
-Example sum_vo_v1 : list_bits_to_nat v0_plus_v1 = 21.
+Definition v0_plus_v1 : Bvector 8 := combinational (adderTree 0 v0_v1).
+
+Example sum_vo_v1 : combinational (adderTree2 v0_v1) = N2Bv_sized 8 21.
 Proof. reflexivity. Qed.
 
 (* An adder tree with 4 inputs. *)
 
-Definition adderTree4 {m bit} `{Cava m bit} (v : list (list bit)) : m (list bit)
+Definition adderTree4 {m bit} `{Cava m bit} {sz}
+                      (v : vec (BitVec Bit sz) 4) : m (vec Bit sz)
   := adderTree 1 v.
 
-Definition v0_v1_v2_v3 := [v0; v1; v2; v3].
-Definition adderTree4_v0_v1_v2_v3 : list bool := combinational (adderTree4 v0_v1_v2_v3).
-Example sum_v0_v1_v2_v3 : list_bits_to_nat (combinational (adderTree4 v0_v1_v2_v3)) = 30.
-Proof. reflexivity. Qed.
+Definition v0_3 := [v0; v1; v2; v3].
+Definition sum_v0_3 : Bvector 8 := combinational (adderTree4 v0_3).
 
-Local Open Scope nat_scope.
+Example sum_v0_v1_v2_v3 : combinational (adderTree4 v0_3) = N2Bv_sized 8 30.
+Proof. reflexivity. Qed.
 
 Definition adder_tree_Interface name nrInputs bitSize
   := combinationalInterface name
-     (mkPort "inputs" (BitVec [nrInputs; bitSize]))
-     (mkPort "sum" (BitVec [bitSize + Nat.log2_up nrInputs]))
+     (mkPort "inputs" (BitVec (BitVec Bit bitSize) nrInputs))
+     (mkPort "sum" (BitVec Bit bitSize))
      [].
 
 (* Create netlist and test-bench for a 4-input adder tree. *)
@@ -89,8 +108,11 @@ Definition adder_tree4_8Netlist
 Local Open Scope N_scope.
 
 Definition adder_tree4_8_tb_inputs
-  := map (fun i => map (nat_to_list_bits_sized 8) i)
-     [[17; 42; 23; 95]; [4; 13; 200; 30]; [255; 74; 255; 200]].
+  := map (fun i => Vector.map (N2Bv_sized 8) i)
+     [[17;  42;  23;  95];
+      [ 4;  13; 200;  30]; 
+      [255; 74; 255; 200]
+     ].
 
 Definition adder_tree4_8_tb_expected_outputs
   := map (fun i => combinational (adderTree4 i)) adder_tree4_8_tb_inputs.
@@ -101,22 +123,24 @@ Definition adder_tree4_8_tb :=
 
 (* Create netlist for a 32-input adder tree. *)
 
-Definition adder_tree32_8Interface := adder_tree_Interface "adder_tree32_8" 32 8.
+Definition adder_tree32_8Interface
+  := adder_tree_Interface "adder_tree32_8" 32 8.
 
 Definition adder_tree32_8Netlist
   := makeNetlist adder_tree32_8Interface (adderTree 4).
 
 (* Create netlist and test-bench for a 64-input adder tree. *)
 
-Definition adder_tree64_8Interface := adder_tree_Interface "adder_tree64_8" 64 8.
+Definition adder_tree64_8Interface
+  := adder_tree_Interface "adder_tree64_8" 64 8.
 
 Definition adder_tree64_8Netlist
   := makeNetlist adder_tree64_8Interface (adderTree 5).
 
 Definition adder_tree64_8_tb_inputs
-  := map (fun i => map (nat_to_list_bits_sized 8) i)
-     (repeat 255 64 :: map (map N.of_nat)
-     [seq 0 64; seq 64 64; seq 128 64]).
+  := map (Vector.map (N2Bv_sized 8))
+     (Vector.const 255 64 :: map (Vector.map N.of_nat)
+     [vseq 0 64; vseq 64 64; vseq 128 64]).
 
 Definition adder_tree64_8_tb_expected_outputs
   := map (fun i => combinational (adderTree 5 i)) adder_tree64_8_tb_inputs.
@@ -133,9 +157,9 @@ Definition adder_tree64_128Netlist
   := makeNetlist adder_tree64_128Interface (adderTree 5).
 
 Definition adder_tree64_128_tb_inputs
-  := map (fun i => map (nat_to_list_bits_sized 128) i)
-     (repeat (2^128-1) 64 :: map (map N.of_nat)
-     [seq 0 64; seq 64 64; seq 128 64]).
+  := map (Vector.map (N2Bv_sized 128))
+     (Vector.const (2^128-1) 64 :: map (Vector.map N.of_nat)
+     [vseq 0 64; vseq 64 64; vseq 128 64]).
 
 Definition adder_tree64_128_tb_expected_outputs
   := map (fun i => combinational (adderTree 5 i)) adder_tree64_128_tb_inputs.
