cava/monad-examples/xilinx/XilinxAdderExamples.v
@@ -15,6 +15,7 @@
 (****************************************************************************)
 
 From Coq Require Import Bool.Bool.
+From Coq Require Import NArith.
 From Coq Require Import Ascii String.
 From Coq Require Import Lists.List.
 From Coq Require Import ZArith.
@@ -30,42 +31,37 @@ Require Import Cava.Monad.XilinxAdder.
 (* A few tests to check the unsigned adder.        *)
 (****************************************************************************)
 
-Definition v0   := [0;0;0;0;0;0;0;0].
-Definition v1   := [1;0;0;0;0;0;0;0].
-Definition v2   := [0;1;0;0;0;0;0;0].
-Definition v3   := [1;1;1;1;1;1;1;1].
-Definition v4   := [1;0;0;0;0;0;0;0].
-Definition v5   := [1;1;1;1;1;1;1;1].
-Definition v6   := [1;1;1;1;1;1;1;1].
-Definition v255 := [1;1;1;1;1;1;1;1].
-
-Definition eval_xilinxAdder cin a b :=
-  let '(sum, carry)
-    := combinational
-       (xilinxAdderWithCarry (nat2bool cin, (toVec a, toVec b))) in
-  (fromVec sum, Nat.b2n carry).
+Definition v17  := N2Bv_sized 8 17.
+Definition v52  := N2Bv_sized 8 52.
+Definition v69  := N2Bv_sized 8 69.
+Definition v70  := N2Bv_sized 8 70.
+Definition v1   := N2Bv_sized 8 1.
+Definition v255 := N2Bv_sized 8 255.
+Definition v0   := N2Bv_sized 8 0.
+Definition v200 := N2Bv_sized 8 200.
+Definition v100 := N2Bv_sized 8 100.
+Definition v44  := N2Bv_sized 8 44.
 
 (* Perform a few basic checks to make sure the adder works. *)
 
-Example v1_plus_v2 : eval_xilinxAdder 0 v1 v2 = ([1; 1; 0; 0; 0; 0; 0; 0], 0).
+Example xadd_17_52_0 : combinational (xilinxAdderWithCarry (false, (v17, v52))) =
+                                     (v69, false).
 Proof. reflexivity. Qed.
 
-Example v0_plus_v1 : eval_xilinxAdder 0 v0 v1 = ([1; 0; 0; 0; 0; 0; 0; 0], 0).
+Example xadd_17_52_1 : combinational (xilinxAdderWithCarry (true, (v17, v52))) =
+                                     (v70, false).
 Proof. reflexivity. Qed.
 
-Example v255_plus_v1 : eval_xilinxAdder 0 v255 v1 = ([0; 0; 0; 0; 0; 0; 0; 0], 1).
+Example xadd_1_255_1 : combinational (xilinxAdderWithCarry (false, (v1, v255))) =
+                                     (v0, true).
 Proof. reflexivity. Qed.
 
-Example v255_plus_v0_cin1 : eval_xilinxAdder 1 v255 v0 = ([0; 0; 0; 0; 0; 0; 0; 0], 1).
+Example xadd_0_255_1 : combinational (xilinxAdderWithCarry (true, (v0, v255))) =
+                                     (v0, true).
 Proof. reflexivity. Qed.
 
-Example v255_plus_255_cin1 : eval_xilinxAdder 1 v255 v255 = ([1; 1; 1; 1; 1; 1; 1; 1], 1).
-Proof. reflexivity. Qed.
-
-Example v3_plus_v4 : eval_xilinxAdder 0 v3 v4 = ([0; 0; 0; 0; 0; 0; 0; 0], 1).
-Proof. reflexivity. Qed.
-
-Example v5_plus_v6 : eval_xilinxAdder 0 v5 v6 = ([0; 1; 1; 1; 1; 1; 1; 1], 1).
+Example xadd_200_100_0 : combinational (xilinxAdderWithCarry (false, (v200, v100))) =
+                                       (v44, true).
 Proof. reflexivity. Qed.
 
 (****************************************************************************)
@@ -75,8 +71,8 @@ Proof. reflexivity. Qed.
 
 Definition adder8Interface
   := combinationalInterface "adder8"
-     (mkPort "cin" Bit, (mkPort "a" (BitVec [8]), mkPort "b" (BitVec [8])))
-     (mkPort "sum" (BitVec [8]), mkPort "cout" Bit)
+     (mkPort "cin" Bit, (mkPort "a" (BitVec Bit 8), mkPort "b" (BitVec Bit 8)))
+     (mkPort "sum" (BitVec Bit 8), mkPort "cout" Bit)
      [].
 
 Definition adder8Netlist := makeNetlist adder8Interface xilinxAdderWithCarry.
@@ -85,7 +81,7 @@ Local Open Scope N_scope.
 
 Definition adder8_tb_inputs :=
   map (fun '(cin, (a, b))
-       => (n2bool cin, (nat_to_list_bits_sized 8 a, nat_to_list_bits_sized 8 b)))
+       => (n2bool cin, (N2Bv_sized 8 a, N2Bv_sized 8 b)))
   [(0, (7, 3));
    (1, (115, 67));
    (0, (92, 18));
