cava/monad-examples/xilinx/XilinxAdderTree.v
@@ -14,17 +14,17 @@
 (* limitations under the License.                                           *)
 (****************************************************************************)
 
-(* A codification of the Lava embedded DSL develope for Haskell into
-   Coq for the specification, implementaiton and formal verification of
-   circuits. Experimental work, very much in flux, as Satnam learns Coq!
-*)
-
 From Coq Require Import Bool.Bool.
 From Coq Require Import Ascii String.
+From Coq Require Import NArith.
 Require Import Omega.
 
 From Coq Require Import Lists.List.
 Import ListNotations.
+
+From Coq Require Import Vector.
+From Coq Require Import Bool.Bvector.
+Import VectorNotations.
 
 Require Import ExtLib.Structures.Monads.
 
@@ -37,16 +37,20 @@ Require Import Cava.Monad.XilinxAdder.
 (* by using the tree combinator.                                              *)
 (******************************************************************************)
 
-Definition adderTree {m bit} `{Cava m bit} := tree xilinxAdder.
+Definition adderTree {m bit vec} `{Cava m bit vec} {sz: nat}
+                     (n: nat) (v: vec (BitVec Bit (S sz)) (2^(n+1))) :
+                     m (vec Bit (S sz)) :=
+  let vv : Vector.t (vec Bit (S sz)) (2^(n+1)) := vecToVector2 Bit (S sz) v in 
+  tree xilinxAdder defaultBitVec n vv.
 
 (******************************************************************************)
 (* Some tests.                                                                *)
 (******************************************************************************)
 
-Definition v0 := nat_to_list_bits_sized 8  4.
-Definition v1 := nat_to_list_bits_sized 8 17.
-Definition v2 := nat_to_list_bits_sized 8  6.
-Definition v3 := nat_to_list_bits_sized 8  3.
+Definition v0 := N2Bv_sized 8  4.
+Definition v1 := N2Bv_sized 8 17.
+Definition v2 := N2Bv_sized 8  6.
+Definition v3 := N2Bv_sized 8  3.
 
 Local Open Scope N_scope.
 Local Open Scope string_scope.
@@ -55,37 +59,44 @@ Local Open Scope string_scope.
 (* An adder tree with 2 inputs.                                               *)
 (******************************************************************************)
 
-Definition adderTree2 {m bit} `{Cava m bit} (v : list (list bit)) : m (list bit)
+Local Open Scope nat_scope.
+Local Open Scope vector_scope.
+
+Definition adderTree2 {m bit vec} `{Cava m bit vec} {sz}
+                      (v : vec (BitVec Bit (S sz)) 2) : m (vec Bit (S sz))
   := adderTree 0 v.
 
-Definition v0_v1 := [v0; v1].
-Definition v0_plus_v1 : list bool := combinational (adderTree 0 v0_v1).
-Example sum_vo_v1 : list_bits_to_nat v0_plus_v1 = 21.
+Definition v0_v1 : Vector.t (Bvector 8) 2 := [v0; v1].
+Definition v0_plus_v1 : Bvector 8 := combinational (adderTree2 v0_v1).
+Example sum_vo_v1 : v0_plus_v1 = N2Bv_sized 8 21.
 Proof. reflexivity. Qed.
 
 (******************************************************************************)
 (* An adder tree with 4 inputs.                                               *)
 (******************************************************************************)
 
-Definition adderTree4 {m bit} `{Cava m bit} (v : list (list bit)) : m (list bit)
+Definition adderTree4 {m bit} `{Cava m bit} {sz}
+                      (v : vec (BitVec Bit (S sz)) 4) : m (vec Bit (S sz))
   := adderTree 1 v.
 
+Local Open Scope N_scope.
+
 Definition v0_v1_v2_v3 := [v0; v1; v2; v3].
-Definition adderTree4_v0_v1_v2_v3 : list bool := combinational (adderTree4 v0_v1_v2_v3).
-Example sum_v0_v1_v2_v3 : list_bits_to_nat (combinational (adderTree4 v0_v1_v2_v3)) = 30.
+Definition adderTree4_v0_v1_v2_v3 := combinational (adderTree4 v0_v1_v2_v3).
+Example sum_v0_v1_v2_v3 : Bv2N (combinational (adderTree4 v0_v1_v2_v3)) = 30.
 Proof. reflexivity. Qed.
 
 Local Open Scope nat_scope.
 
-Definition adder_tree_Interface name degree bitSize
+Definition adder_tree_Interface name nrInputs bitSize
   := combinationalInterface name
-     (mkPort "inputs" (BitVec [2^(degree + 1); bitSize]))
-     (mkPort "sum" (BitVec [bitSize + degree + 1]))
+     (mkPort "inputs" (BitVec (BitVec Bit bitSize) nrInputs))
+     (mkPort "sum" (BitVec Bit bitSize))
      [].
 
 (* Create netlist and test-bench for a 4-input adder tree. *)
 
-Definition adder_tree4_8Interface := adder_tree_Interface "xadder_tree4_8" 1 8.
+Definition adder_tree4_8Interface := adder_tree_Interface "xadder_tree4_8" 4 8.
 
 Definition adder_tree4_8Netlist
   := makeNetlist adder_tree4_8Interface adderTree4.
@@ -93,8 +104,8 @@ Definition adder_tree4_8Netlist
 Local Open Scope N_scope.
 
 Definition adder_tree4_8_tb_inputs
-  := map (fun i => map (nat_to_list_bits_sized 8) i)
-     (repeat (2^8-1) 4 ::
+  := map (fun i => Vector.map (N2Bv_sized 8) i)
+     (Vector.const (2^8-1) 4 ::
      [[17; 42; 23; 95]; [4; 13; 200; 30]; [255; 74; 255; 200]; [44; 12; 92; 12];
       [9; 56; 2; 87];   [14; 72; 90; 11]; [64; 12; 92; 13];    [88; 24; 107; 200]]).
 
@@ -108,29 +119,29 @@ Definition adder_tree4_8_tb :=
 (* Test to make sure this instance of the adder tree produces
    the expected output for the test bench case. *)
 Example adder_tree_4_8_test:
-   map list_bits_to_nat adder_tree4_8_tb_expected_outputs
-   = [1020; 177; 247; 784; 160; 154; 187; 181; 419].
+   map Bv2N adder_tree4_8_tb_expected_outputs
+   = [252; 177; 247; 16; 160; 154; 187; 181; 163]%list.
 Proof. reflexivity. Qed.
 
 (******************************************************************************)
 (* Create netlist for a 32-input adder tree.                                  *)
 (******************************************************************************)
 
-Definition adder_tree32_8Interface := adder_tree_Interface "xadder_tree32_8" 4 8.
+Definition adder_tree32_8Interface := adder_tree_Interface "xadder_tree32_8" 32 8.
 
 Definition adder_tree32_8Netlist
   := makeNetlist adder_tree32_8Interface (adderTree 4).
 
 (* Create netlist and test-bench for a 64-input adder tree. *)
 
-Definition adder_tree64_8Interface := adder_tree_Interface "xadder_tree64_8" 5 8.
+Definition adder_tree64_8Interface := adder_tree_Interface "xadder_tree64_8" 64 8.
 
 Definition adder_tree64_8Netlist
   := makeNetlist adder_tree64_8Interface (adderTree 5).
 
 Definition adder_tree64_8_tb_inputs
-  := map (fun i => map (nat_to_list_bits_sized 8) (map N.of_nat i))
-     [seq 0 64; seq 64 64; seq 128 64].
+  := map (fun i => Vector.map (N2Bv_sized 8) (Vector.map N.of_nat i))
+     [vseq 0 64; vseq 64 64; vseq 128 64].
 
 Definition adder_tree64_8_tb_expected_outputs
   := map (fun i => combinational (adderTree 5 i)) adder_tree64_8_tb_inputs.
@@ -143,17 +154,15 @@ Definition adder_tree64_8_tb :=
 (* Create netlist and test-bench for a 64-input adder of 128-bit inputs       *)
 (******************************************************************************)
 
-Definition adder_tree64_128Interface := adder_tree_Interface "xadder_tree64_128" 5 128.
+Definition adder_tree64_128Interface := adder_tree_Interface "xadder_tree64_128" 64 128.
 
 Definition adder_tree64_128Netlist
   := makeNetlist adder_tree64_128Interface (adderTree 5).
 
-Local Open Scope N_scope.
-
 Definition adder_tree64_128_tb_inputs
-  := map (fun i => map (nat_to_list_bits_sized 128) i)
-     (repeat (2^128-1) 64 :: map (map N.of_nat)
-     [seq 0 64; seq 64 64; seq 128 64]).
+  := map (fun i => Vector.map (N2Bv_sized 128) i)
+     (Vector.const (2^128-1) 64 :: map (Vector.map N.of_nat)
+     [vseq 0 64; vseq 64 64; vseq 128 64]).
 
 Definition adder_tree64_128_tb_expected_outputs
   := map (fun i => combinational (adderTree 5 i)) adder_tree64_128_tb_inputs.
@@ -166,18 +175,19 @@ Definition adder_tree64_128_tb :=
 (* Create netlist and test-bench for a 128-input adder of 256-bit inputs      *)
 (******************************************************************************)
 
-Definition adder_tree128_256Interface := adder_tree_Interface "xadder_tree128_256" 6 256.
+Definition adder_tree128_256Interface := adder_tree_Interface "xadder_tree128_256" 128 256.
 
 Definition adder_tree128_256Netlist
   := makeNetlist adder_tree128_256Interface (adderTree 6).
 
-Definition adder_tree128_256_tb_inputs
-  := map (fun i => map (nat_to_list_bits_sized 256) i)
-     (repeat (2^256-1) 128 :: map (map N.of_nat)
-     [seq 0 128; seq 128 128; seq 256 128]).
+Definition adder_tree128_256_tb_inputs : list (Vector.t (Bvector 256) 128)
+  := map (fun i => Vector.map (N2Bv_sized 256) i)
+     (Vector.const (2^256-1) 128 :: map (Vector.map N.of_nat)
+     [vseq 0 128; vseq 128 128; vseq 256 128]).
 
 Definition adder_tree128_256_tb_expected_outputs
-  := map (fun i => combinational (adderTree 5 i)) adder_tree64_128_tb_inputs.
+           : list (Bvector 256)
+  := map (fun i => combinational (adderTree 6 i)) adder_tree128_256_tb_inputs.
 
 Definition adder_tree128_256_tb :=
   testBench "xadder_tree128_256_tb" adder_tree128_256Interface
