cava/cava/Cava/Cava.v
@@ -21,4 +21,6 @@
 
 Require Export Cava.BitArithmetic.
 Require Export Cava.Netlist.
+Require Export Cava.Kind.
 Require Export Cava.Types.
+Require Export Cava.VectorUtils.
