cava/cava/Cava/Monad/UnsignedAdders.v
@@ -16,16 +16,37 @@
 
 Require Import ExtLib.Structures.Monads.
 
+Require Import Nat Arith Lia.
+
 Require Import Cava.Cava.
+From Cava Require Import Kind.
 Require Import Cava.Monad.CavaMonad.
+
+(******************************************************************************)
+(* An adder with two inputs of the same size and no bit-growth                *)
+(******************************************************************************)
+
+Lemma n_le_max_n_n : forall n, n <= S(max n n).
+Proof.
+  intros. lia.
+Qed.
+
+Definition addN {m bit} `{Cava m bit} {n}
+                (a: vec Bit n) (b: vec Bit n) : m (vec Bit n) :=
+  s <- unsignedAdd a b ;;
+  ret (slice 0 n s (n_le_max_n_n n)).
 
 (******************************************************************************)
 (* A three input adder.                                                       *)
 (******************************************************************************)
 
 Definition adder_3input {m bit} `{Cava m bit}
-                        (a : list bit) (b : list bit) (c : list bit)
-                        : m (list bit) :=
+                        {aSize bSize cSize}
+                        (a : vec Bit aSize)
+                        (b : vec Bit bSize)
+                        (c : vec Bit cSize) :
+                        m (vec Bit (1 + max (1 + max aSize bSize) cSize))
+                        :=
   a_plus_b <- unsignedAdd a b ;;
   sum <- unsignedAdd a_plus_b c ;;
   ret sum.
